src/Compilers/Z/Bounds/InterpretationLemmas.v
@@ -15,9 +15,6 @@ Require Import Crypto.Util.Tactics.SpecializeBy.
 Require Import Crypto.Util.Tactics.SplitInContext.
 Require Import Crypto.Util.Tactics.UniquePose.
 
-Local Notation pick_typeb := Bounds.bounds_to_base_type (only parsing).
-Local Notation pick_type v := (SmartFlatTypeMap (fun _ => pick_typeb) v).
-
 Local Open Scope Z_scope.
 
 Local Ltac break_t_step :=
@@ -232,7 +229,7 @@ Lemma is_bounded_by_truncation_bounds Tout bs v
                          (Bounds.truncation_bounds (Bounds.bit_width_of_base_type Tout) bs)
                          (ZToInterp v).
 Proof.
-  destruct bs as [l u]; cbv [Bounds.truncation_bounds Bounds.is_bounded_by Bounds.is_bounded_by' Bounds.bit_width_of_base_type ZRange.is_bounded_by'] in *; simpl in *.
+  destruct bs as [l u]; cbv [Bounds.truncation_bounds Bounds.is_bounded_by Bounds.is_bounded_by' Bounds.bit_width_of_base_type Bounds.log_bit_width_of_base_type option_map ZRange.is_bounded_by'] in *; simpl in *.
   repeat first [ break_t_step
                | fin_t
                | progress simpl in *
@@ -304,130 +301,136 @@ Local Arguments unzify_op : simpl never.
 Local Arguments Z.pow : simpl never.
 Local Arguments Z.add !_ !_.
 Local Existing Instance Z.pow_Zpos_le_Proper.
-Lemma pull_cast_genericize_op t tR (opc : op t tR)
-      (bs : interp_flat_type Bounds.interp_base_type t)
-      (v : interp_flat_type interp_base_type (pick_type bs))
-      (H : Bounds.is_bounded_by bs
-                                (SmartFlatTypeMapUnInterp
-                                   (fun (t1 : base_type) (b0 : Bounds.interp_base_type t1) => cast_const) v))
-  : interp_op t tR opc (cast_back_flat_const v)
-    = cast_back_flat_const (interp_op (pick_type bs) (pick_type (Bounds.interp_op opc bs)) (genericize_op opc) v).
-Proof.
-  pose proof (is_bounded_by_interp_op t tR opc bs).
-  unfold interp_op in *.
-  rewrite Zinterp_op_genericize_op.
-  generalize dependent (Zinterp_op t tR opc).
-  generalize dependent (Bounds.interp_op opc bs); clear opc; simpl; intros.
-  revert dependent t; induction tR as [tR| |]; intros;
-    [
-    | repeat first [ match goal with
-                     | [ |- ?x = ?y ]
-                       => transitivity tt; destruct x, y; reflexivity
-                     end
-                   | reflexivity
-                   | progress simpl @Bounds.is_bounded_by in *
-                   | rewrite !lift_op_prod_dst
-                   | rewrite !cast_back_flat_const_prod
-                   | progress split_and
-                   | match goal with
-                     | [ H : _ |- _ ] => first [ setoid_rewrite lift_op_prod_dst in H
-                                               | setoid_rewrite cast_back_flat_const_prod in H ]
-                     end
-                   | setoid_rewrite lift_op_prod_dst
-                   | match goal with
-                     | [ H : _ |- _ ] => erewrite H by eassumption
-                     end ].. ].
-  revert dependent tR; induction t as [t| |]; intros;
-    [
-    | repeat first [ match goal with
-                     | [ |- ?x = ?y ]
-                       => transitivity tt; destruct x, y; reflexivity
-                     end
-                   | reflexivity
-                   | progress simpl @Bounds.is_bounded_by in *
-                   | rewrite !lift_op_prod_dst
-                   | rewrite !cast_back_flat_const_prod
-                   | progress split_and
-                   | match goal with
-                     | [ H : _ |- _ ] => first [ setoid_rewrite lift_op_prod_dst in H
-                                               | setoid_rewrite cast_back_flat_const_prod in H ]
-                     end
-                   | setoid_rewrite lift_op_prod_dst
-                   | match goal with
-                     | [ H : _ |- _ ] => erewrite H by eassumption
-                     end ].. ].
-  { simpl in *; unfold unzify_op, cast_back_flat_const, SmartFlatTypeMap, Bounds.interp_base_type, cast_const, Bounds.is_bounded_by', lift_op, SmartFlatTypeMapUnInterp, SmartFlatTypeMapInterp2, cast_const in *; simpl in *.
-    unfold Bounds.is_bounded_by', cast_const, ZToInterp, interpToZ, Bounds.bounds_to_base_type, ZRange.is_bounded_by' in *; simpl in *.
-    destruct_head base_type; break_innermost_match; Z.ltb_to_lt; destruct_head Bounds.t;
-      repeat match goal with
-             | _ => progress destruct_head'_and
-             | _ => reflexivity
-             | [ H : forall v, _ /\ True -> _ |- _ ] => specialize (fun v pf => H v (conj pf I))
-             | [ H : forall v, _ -> _ /\ True |- _ ] => pose proof (fun v pf => proj1 (H v pf)); clear H
-             | [ H : True |- _ ] => clear H
-             | [ H : ?T, H' : ?T |- _ ] => clear H
-             | [ H : forall v, _ -> _ <= ?f v <= _ |- ?f ?v' = _ ]
-               => specialize (H v')
-             | [ H : forall v, _ -> _ <= ?f (?g v) <= _ |- ?f (?g ?v') = _ ]
-               => specialize (H v')
-             | [ H : forall v, _ -> _ <= ?f (?g (?h v)) <= _ /\ _ /\ _ |- context[?h ?v'] ]
-               => specialize (H v')
-             | [ H : forall v, _ -> _ <= ?f (?g (?h (?i v))) <= _ /\ _ /\ _ |- context[?h (?i ?v')] ]
-               => specialize (H v')
-             | _ => progress specialize_by omega
-             | _ => rewrite wordToZ_ZToWord
-                 by repeat match goal with
-                           | [ |- and _ _ ] => split
-                           | [ |- ?x < ?y ] => cut (1 + x <= y); [ omega | ]
-                           | _ => omega
-                           | _ => progress autorewrite with push_Zof_nat zsimplify_const
-                           | _ => rewrite Z2Nat.id by auto with zarith
-                           | _ => rewrite <- !Z.log2_up_le_full
-                           end
-             | _ => rewrite wordToZ_ZToWord in *
-                 by repeat match goal with
-                           | [ |- and _ _ ] => split
-                           | [ |- ?x < ?y ] => cut (1 + x <= y); [ omega | ]
-                           | _ => omega
-                           | _ => progress autorewrite with push_Zof_nat zsimplify_const
-                           | _ => rewrite Z2Nat.id by auto with zarith
-                           | _ => rewrite <- !Z.log2_up_le_full
-                           end
-             | _ => rewrite wordToZ_ZToWord_wordToZ
-                 by (rewrite Nat2Z.inj_le, Z2Nat.id, <- !Z.log2_up_le_pow2_full by auto with zarith; omega)
-             | _ => rewrite wordToZ_ZToWord_wordToZ in *
-                 by (rewrite Nat2Z.inj_le, Z2Nat.id, <- !Z.log2_up_le_pow2_full by auto with zarith; omega)
-             end.
-    all:admit. }
-  { simpl in *.
-    specialize (H0 tt I).
-    simpl in *.
-    hnf in H0.
-    unfold cast_back_flat_const, lift_op, unzify_op in *; simpl in *.
-    unfold interpToZ in *.
-    unfold Bounds.bounds_to_base_type in *.
-    destruct_head base_type; simpl in *.
-    split_andb.
-    Z.ltb_to_lt.
-    all:destruct_head' and.
-    all:simpl in *.
-    all:break_innermost_match; break_match_hyps; split_andb; Z.ltb_to_lt; try reflexivity.
-    all:try (simpl in *;
-    rewrite wordToZ_ZToWord
-      by (autorewrite with push_Zof_nat zsimplify_const;
-        rewrite Z2Nat.id by auto with zarith;
-        split; try omega;
-        match goal with
-        | [ |- (?x < ?y)%Z ]
-          => apply (Z.lt_le_trans x (x + 1) y); [ omega | ]
-        end;
-        rewrite <- !Z.log2_up_le_full;
-        omega)).
-    all:try reflexivity.
-    unfold interpToZ, cast_const.
-    simpl.
-    rewrite ZToWord_wordToZ_ZToWord; [ reflexivity | ].
-    apply Nat2Z.inj_le.
-    rewrite Z2Nat.id by auto with zarith.
 
-Admitted.
+Section with_round_up.
+  Context {round_up : nat -> option nat}.
+
+  Local Notation pick_typeb := (@Bounds.bounds_to_base_type round_up) (only parsing).
+  Local Notation pick_type v := (SmartFlatTypeMap pick_typeb v).
+
+  Lemma pull_cast_genericize_op
+        t tR (opc : op t tR)
+        (bs : interp_flat_type Bounds.interp_base_type t)
+        (v : interp_flat_type interp_base_type (pick_type bs))
+        (H : Bounds.is_bounded_by bs
+                                  (SmartFlatTypeMapUnInterp
+                                     (fun (t1 : base_type) (b0 : Bounds.interp_base_type t1) => cast_const) v))
+    : interp_op t tR opc (cast_back_flat_const v)
+      = cast_back_flat_const (interp_op (pick_type bs) (pick_type (Bounds.interp_op opc bs)) (genericize_op opc) v).
+  Proof.
+    pose proof (is_bounded_by_interp_op t tR opc bs).
+    unfold interp_op in *.
+    rewrite Zinterp_op_genericize_op.
+    generalize dependent (Zinterp_op t tR opc).
+    generalize dependent (Bounds.interp_op opc bs); clear opc; simpl; intros.
+    revert dependent t; induction tR as [tR| |]; intros;
+      [
+      | repeat first [ match goal with
+                       | [ |- ?x = ?y ]
+                         => transitivity tt; destruct x, y; reflexivity
+                       end
+                     | reflexivity
+                     | progress simpl @Bounds.is_bounded_by in *
+                     | rewrite !lift_op_prod_dst
+                     | rewrite !cast_back_flat_const_prod
+                     | progress split_and
+                     | match goal with
+                       | [ H : _ |- _ ] => first [ setoid_rewrite lift_op_prod_dst in H
+                                                 | setoid_rewrite cast_back_flat_const_prod in H ]
+                       end
+                     | setoid_rewrite lift_op_prod_dst
+                     | match goal with
+                       | [ H : _ |- _ ] => erewrite H by eassumption
+                       end ].. ].
+    revert dependent tR; induction t as [t| |]; intros;
+      [
+      | repeat first [ match goal with
+                       | [ |- ?x = ?y ]
+                         => transitivity tt; destruct x, y; reflexivity
+                       end
+                     | reflexivity
+                     | progress simpl @Bounds.is_bounded_by in *
+                     | rewrite !lift_op_prod_dst
+                     | rewrite !cast_back_flat_const_prod
+                     | progress split_and
+                     | match goal with
+                       | [ H : _ |- _ ] => first [ setoid_rewrite lift_op_prod_dst in H
+                                                 | setoid_rewrite cast_back_flat_const_prod in H ]
+                       end
+                     | setoid_rewrite lift_op_prod_dst
+                     | match goal with
+                       | [ H : _ |- _ ] => erewrite H by eassumption
+                       end ].. ].
+    { simpl in *; unfold unzify_op, cast_back_flat_const, SmartFlatTypeMap, Bounds.interp_base_type, cast_const, Bounds.is_bounded_by', lift_op, SmartFlatTypeMapUnInterp, SmartFlatTypeMapInterp2, cast_const in *; simpl in *.
+      unfold Bounds.is_bounded_by', cast_const, ZToInterp, interpToZ, Bounds.bounds_to_base_type, ZRange.is_bounded_by' in *; simpl in *.
+      destruct_head base_type; break_innermost_match; Z.ltb_to_lt; destruct_head Bounds.t;
+        repeat match goal with
+               | _ => progress destruct_head'_and
+               | _ => reflexivity
+               | [ H : forall v, _ /\ True -> _ |- _ ] => specialize (fun v pf => H v (conj pf I))
+               | [ H : forall v, _ -> _ /\ True |- _ ] => pose proof (fun v pf => proj1 (H v pf)); clear H
+               | [ H : True |- _ ] => clear H
+               | [ H : ?T, H' : ?T |- _ ] => clear H
+               | [ H : forall v, _ -> _ <= ?f v <= _ |- ?f ?v' = _ ]
+                 => specialize (H v')
+               | [ H : forall v, _ -> _ <= ?f (?g v) <= _ |- ?f (?g ?v') = _ ]
+                 => specialize (H v')
+               | [ H : forall v, _ -> _ <= ?f (?g (?h v)) <= _ /\ _ /\ _ |- context[?h ?v'] ]
+                 => specialize (H v')
+               | [ H : forall v, _ -> _ <= ?f (?g (?h (?i v))) <= _ /\ _ /\ _ |- context[?h (?i ?v')] ]
+                 => specialize (H v')
+               | _ => progress specialize_by omega
+               | _ => rewrite wordToZ_ZToWord
+                   by repeat match goal with
+                             | [ |- and _ _ ] => split
+                             | [ |- ?x < ?y ] => cut (1 + x <= y); [ omega | ]
+                             | _ => omega
+                             | _ => progress autorewrite with push_Zof_nat zsimplify_const
+                             | _ => rewrite Z2Nat.id by auto with zarith
+                             | _ => rewrite <- !Z.log2_up_le_full
+                             end
+               | _ => rewrite wordToZ_ZToWord in *
+                   by repeat match goal with
+                             | [ |- and _ _ ] => split
+                             | [ |- ?x < ?y ] => cut (1 + x <= y); [ omega | ]
+                             | _ => omega
+                             | _ => progress autorewrite with push_Zof_nat zsimplify_const
+                             | _ => rewrite Z2Nat.id by auto with zarith
+                             | _ => rewrite <- !Z.log2_up_le_full
+                             end
+               | _ => rewrite wordToZ_ZToWord_wordToZ
+                   by (rewrite Nat2Z.inj_le, Z2Nat.id, <- !Z.log2_up_le_pow2_full by auto with zarith; omega)
+               | _ => rewrite wordToZ_ZToWord_wordToZ in *
+                   by (rewrite Nat2Z.inj_le, Z2Nat.id, <- !Z.log2_up_le_pow2_full by auto with zarith; omega)
+               end.
+      all:admit. }
+    { simpl in *.
+      specialize (H0 tt I).
+      simpl in *.
+      hnf in H0.
+      unfold cast_back_flat_const, lift_op, unzify_op in *; simpl in *.
+      unfold interpToZ in *.
+      unfold Bounds.bounds_to_base_type in *.
+      destruct_head base_type; simpl in *.
+      split_andb.
+      Z.ltb_to_lt.
+      all:destruct_head' and.
+      all:simpl in *.
+      all:break_innermost_match; break_match_hyps; split_andb; Z.ltb_to_lt; try reflexivity.
+      all:try (simpl in *;
+               rewrite wordToZ_ZToWord
+                 by (autorewrite with push_Zof_nat zsimplify_const;
+                     rewrite Z2Nat.id by auto with zarith;
+                     split; try omega;
+                     match goal with
+                     | [ |- (?x < ?y)%Z ]
+                       => apply (Z.lt_le_trans x (x + 1) y); [ omega | ]
+                     end;
+                     rewrite <- !Z.log2_up_le_full;
+                     omega)).
+      all:try reflexivity.
+      unfold interpToZ, cast_const.
+      simpl.
+
+  Admitted.
+End with_round_up.
