src/Compilers/Z/Bounds/MapCastByDeBruijn.v
@@ -5,18 +5,19 @@ Require Import Crypto.Compilers.Z.Syntax.Util.
 Require Import Crypto.Compilers.Z.Bounds.Interpretation.
 
 Section language.
-  Context {t : type base_type}.
+  Context (round_up : nat -> option nat)
+          {t : type base_type}.
 
   Definition MapCastCompile := @MapCastCompile t.
   Definition MapCastDoCast
     := @MapCastDoCast
          (@Bounds.interp_base_type) (@Bounds.interp_op)
-         (fun _ => @Bounds.bounds_to_base_type)
+         (@Bounds.bounds_to_base_type round_up)
          (fun _ _ opc _ => @genericize_op _ _ _ opc _ _ _)
          t.
   Definition MapCastDoInterp
     := @MapCastDoInterp
-         (@Bounds.interp_base_type) (fun _ => @Bounds.bounds_to_base_type)
+         (@Bounds.interp_base_type) (@Bounds.bounds_to_base_type round_up)
          t.
   Definition MapCast e input_bounds
     := MapCastDoInterp input_bounds (MapCastDoCast input_bounds (MapCastCompile e)).
