src/Compilers/Z/Bounds/MapCastByDeBruijnInterp.v
@@ -10,10 +10,11 @@ Require Import Crypto.Compilers.Z.Bounds.InterpretationLemmas.
 Require Import Crypto.Compilers.Z.Bounds.MapCastByDeBruijn.
 
 Lemma MapCastCorrect
+      {round_up}
       {t} (e : Expr base_type op t)
       (Hwf : Wf e)
       (input_bounds : interp_flat_type Bounds.interp_base_type (domain t))
-  : forall {b} e' (He':MapCast e input_bounds = Some (existT _ b e'))
+  : forall {b} e' (He':MapCast round_up e input_bounds = Some (existT _ b e'))
            v v' (Hv : Bounds.is_bounded_by input_bounds v /\ cast_back_flat_const v' = v),
     Interp (@Bounds.interp_op) e input_bounds = b
     /\ Bounds.is_bounded_by b (Interp interp_op e v)
