src/Compilers/Z/Bounds/MapCastByDeBruijnWf.v
@@ -10,32 +10,34 @@ Require Import Crypto.Compilers.Z.Bounds.InterpretationLemmas.
 Require Import Crypto.Compilers.Z.Bounds.MapCastByDeBruijn.
 
 Definition Wf_MapCast
+           {round_up}
            {t} (e : Expr base_type op t)
            (input_bounds : interp_flat_type Bounds.interp_base_type (domain t))
-           {b} e' (He' : MapCast e input_bounds = Some (existT _ b e'))
+           {b} e' (He' : MapCast round_up e input_bounds = Some (existT _ b e'))
            (Hwf : Wf e)
   : Wf e'
   := @Wf_MapCast
        (@Bounds.interp_base_type) (@Bounds.interp_op)
-       (fun _ => @Bounds.bounds_to_base_type)
+       (@Bounds.bounds_to_base_type round_up)
        (fun _ _ opc _ => @genericize_op _ _ _ opc _ _ _)
        t e input_bounds b e' He' Hwf.
 
 Definition Wf_MapCast_arrow
+           {round_up}
            {s d} (e : Expr base_type op (Arrow s d))
            (input_bounds : interp_flat_type Bounds.interp_base_type s)
-           {b} e' (He' : MapCast e input_bounds = Some (existT _ b e'))
+           {b} e' (He' : MapCast round_up e input_bounds = Some (existT _ b e'))
            (Hwf : Wf e)
   : Wf e'
   := @Wf_MapCast_arrow
        (@Bounds.interp_base_type) (@Bounds.interp_op)
-       (fun _ => @Bounds.bounds_to_base_type)
+       (@Bounds.bounds_to_base_type round_up)
        (fun _ _ opc _ => @genericize_op _ _ _ opc _ _ _)
        s d e input_bounds b e' He' Hwf.
 
 Hint Extern 1 (Wf ?e')
 => match goal with
-   | [ He : MapCast _ _ = Some (existT _ _ e') |- _ ]
-     => first [ refine (@Wf_MapCast _ _ _ _ _ He _)
-              | refine (@Wf_MapCast_arrow _ _ _ _ _ _ He _) ]
+   | [ He : MapCast _ _ _ = Some (existT _ _ e') |- _ ]
+     => first [ refine (@Wf_MapCast _ _ _ _ _ _ He _)
+              | refine (@Wf_MapCast_arrow _ _ _ _ _ _ _ He _) ]
    end : wf.
