src/Compilers/Z/Bounds/Pipeline/OutputType.v
@@ -7,40 +7,41 @@ Require Import Crypto.Compilers.Z.Syntax.
 Require Import Crypto.Compilers.Z.Bounds.Interpretation.
 Require Import Crypto.Util.Sigma.
 Require Import Crypto.Util.Prod.
-Local Notation pick_typeb := Bounds.bounds_to_base_type (only parsing).
-Local Notation pick_type v := (SmartFlatTypeMap (fun _ => pick_typeb) v).
 
-Record ProcessedReflectivePackage
-  := { InputType : _;
-       input_expr : Expr base_type op InputType;
-       input_bounds : interp_flat_type Bounds.interp_base_type (domain InputType);
-       output_bounds :> interp_flat_type Bounds.interp_base_type (codomain InputType);
-       output_expr :> Expr base_type op (Arrow (pick_type input_bounds) (pick_type output_bounds)) }.
+Section with_round_up_list.
+  Context {allowable_lgsz : list nat}.
 
-Notation OutputType pkg
-  := (Arrow (pick_type (@input_bounds pkg)) (pick_type (@output_bounds pkg)))
-       (only parsing).
+  Local Notation pick_typeb := (@Bounds.bounds_to_base_type (Bounds.round_up_to_in_list allowable_lgsz)) (only parsing).
+  Local Notation pick_type v := (SmartFlatTypeMap pick_typeb v).
 
-Definition Build_ProcessedReflectivePackage_from_option_sigma
-           {t} (e : Expr base_type op t)
-           (input_bounds : interp_flat_type Bounds.interp_base_type (domain t))
-           (result : option { output_bounds : interp_flat_type Bounds.interp_base_type (codomain t)
-                                              & Expr base_type op (Arrow (pick_type input_bounds) (pick_type output_bounds)) })
-  : option ProcessedReflectivePackage
-  := option_map
-       (fun be
-        => let 'existT b e' := be in
-           {| InputType := t ; input_expr := e ; input_bounds := input_bounds ; output_bounds := b ; output_expr := e' |})
-       result.
+  Record ProcessedReflectivePackage
+    := { InputType : _;
+         input_expr : Expr base_type op InputType;
+         input_bounds : interp_flat_type Bounds.interp_base_type (domain InputType);
+         output_bounds :> interp_flat_type Bounds.interp_base_type (codomain InputType);
+         output_expr :> Expr base_type op (Arrow (pick_type input_bounds) (pick_type output_bounds)) }.
 
-Definition ProcessedReflectivePackage_to_sigT (x : ProcessedReflectivePackage)
-  : { InputType : _
-                  & Expr base_type op InputType
-                    * { bounds : interp_flat_type Bounds.interp_base_type (domain InputType)
-                                 * interp_flat_type Bounds.interp_base_type (codomain InputType)
-                                 & Expr base_type op (Arrow (pick_type (fst bounds)) (pick_type (snd bounds))) } }%type
-  := let (a, b, c, d, e) := x in
-     existT _ a (b, (existT _ (c, d) e)).
+  Definition Build_ProcessedReflectivePackage_from_option_sigma
+             {t} (e : Expr base_type op t)
+             (input_bounds : interp_flat_type Bounds.interp_base_type (domain t))
+             (result : option { output_bounds : interp_flat_type Bounds.interp_base_type (codomain t)
+                                                & Expr base_type op (Arrow (pick_type input_bounds) (pick_type output_bounds)) })
+    : option ProcessedReflectivePackage
+    := option_map
+         (fun be
+          => let 'existT b e' := be in
+             {| InputType := t ; input_expr := e ; input_bounds := input_bounds ; output_bounds := b ; output_expr := e' |})
+         result.
+
+  Definition ProcessedReflectivePackage_to_sigT (x : ProcessedReflectivePackage)
+    : { InputType : _
+                    & Expr base_type op InputType
+                      * { bounds : interp_flat_type Bounds.interp_base_type (domain InputType)
+                                   * interp_flat_type Bounds.interp_base_type (codomain InputType)
+                                   & Expr base_type op (Arrow (pick_type (fst bounds)) (pick_type (snd bounds))) } }%type
+    := let (a, b, c, d, e) := x in
+       existT _ a (b, (existT _ (c, d) e)).
+End with_round_up_list.
 
 Ltac inversion_ProcessedReflectivePackage :=
   repeat match goal with
