src/Compilers/Z/Bounds/Pipeline/ReflectiveTactics.v
@@ -148,66 +148,70 @@ Require Import Crypto.Util.PartiallyReifiedProp.
 Require Import Crypto.Util.Equality.
 
 (** *** Gallina assembly *)
-Local Notation pick_typeb := Bounds.bounds_to_base_type (only parsing).
-Local Notation pick_type v := (SmartFlatTypeMap (fun _ => pick_typeb) v).
-Definition PipelineCorrect
-           {t}
-           {input_bounds : interp_flat_type Bounds.interp_base_type (domain t)}
-           {given_output_bounds : interp_flat_type Bounds.interp_base_type (codomain t)}
-           {v' : interp_flat_type Syntax.interp_base_type (pick_type input_bounds)}
-           {b e' e_final e_final_newtype}
-           {fZ}
-           {final_e_evar : interp_flat_type Syntax.interp_base_type (pick_type given_output_bounds)}
-           {e}
-           {e_pkg}
-           (** ** reification *)
-           (rexpr_sig : { rexpr : Expr base_type op t | forall x, Interp Syntax.interp_op rexpr x = fZ x })
-           (** ** pre-wf pipeline *)
-           (He : e = PreWfPipeline (proj1_sig rexpr_sig))
-           (** ** proving wf *)
-           (He_unnatize_for_wf : forall var, unnatize_expr 0 (ExprEta' e (fun t => (nat * var t)%type)) = ExprEta' e _)
-           (Hwf : forall var1 var2,
-               let P := (@reflect_wfT base_type base_type_eq_semidec_transparent op op_beq var1 var2 nil _ _ (ExprEta' e _) (ExprEta' e _)) in
-               trueify P = P)
-           (** ** post-wf-pipeline *)
-           (Hpost : e_pkg = PostWfPipeline e input_bounds)
-           (Hpost_correct : Some {| input_expr := e ; input_bounds := input_bounds ; output_bounds := b ; output_expr := e' |} = e_pkg)
-           (** ** renaming *)
-           (Hrenaming : e_final = e')
-           (** ** bounds relaxation *)
-           (Hbounds_relax : Bounds.is_tighter_thanb b given_output_bounds = true)
-           (Hbounds_sane : pick_type given_output_bounds = pick_type b)
-           (Hbounds_sane_refl
-            : e_final_newtype
-              = eq_rect _ (fun t => Expr base_type op (Arrow (pick_type input_bounds) t)) e' _ (eq_sym Hbounds_sane))
-           (** ** instantiation of original evar *)
-           (Hevar : final_e_evar = InterpEta (t:=Arrow _ _) Syntax.interp_op e_final_newtype v')
-           (** ** side condition *)
-           (Hv : Bounds.is_bounded_by input_bounds (cast_back_flat_const v'))
-  : Bounds.is_bounded_by given_output_bounds (fZ (cast_back_flat_const v'))
-    /\ cast_back_flat_const final_e_evar = fZ (cast_back_flat_const v').
-Proof.
-  destruct rexpr_sig as [? Hrexpr].
-  assert (Hwf' : Wf e)
-    by (apply (proj1 (@Wf_ExprEta'_iff _ _ _ e));
-        eapply reflect_Wf;
-        [ .. | intros; split; [ eapply He_unnatize_for_wf | rewrite <- Hwf; apply trueify_true ] ];
-        auto using base_type_eq_semidec_is_dec, op_beq_bl).
-  clear Hwf He_unnatize_for_wf.
-  symmetry in Hpost_correct.
-  subst; cbv [proj1_sig] in *.
-  rewrite eq_InterpEta, <- Hrexpr.
-  eapply PostWfPipelineCorrect in Hpost_correct; [ | solve [ eauto ].. ].
-  rewrite !@InterpPreWfPipeline in Hpost_correct.
-  unshelve eapply relax_output_bounds; try eassumption; [].
-  match goal with
-  | [ |- context[Interp _ (@eq_rect ?A ?x ?P ?k ?y ?pf) ?v] ]
-    => rewrite (@ap_transport A P _ x y pf (fun t e => Interp interp_op e v) k)
-  end.
-  rewrite <- transport_pp, concat_Vp; simpl.
-  apply Hpost_correct.
-Qed.
+Section with_round_up_list.
+  Context {allowable_lgsz : list nat}.
 
+  Local Notation pick_typeb := (@Bounds.bounds_to_base_type (Bounds.round_up_to_in_list allowable_lgsz)) (only parsing).
+  Local Notation pick_type v := (SmartFlatTypeMap pick_typeb v).
+
+  Definition PipelineCorrect
+             {t}
+             {input_bounds : interp_flat_type Bounds.interp_base_type (domain t)}
+             {given_output_bounds : interp_flat_type Bounds.interp_base_type (codomain t)}
+             {v' : interp_flat_type Syntax.interp_base_type (pick_type input_bounds)}
+             {b e' e_final e_final_newtype}
+             {fZ}
+             {final_e_evar : interp_flat_type Syntax.interp_base_type (pick_type given_output_bounds)}
+             {e}
+             {e_pkg}
+             (** ** reification *)
+             (rexpr_sig : { rexpr : Expr base_type op t | forall x, Interp Syntax.interp_op rexpr x = fZ x })
+             (** ** pre-wf pipeline *)
+             (He : e = PreWfPipeline (proj1_sig rexpr_sig))
+             (** ** proving wf *)
+             (He_unnatize_for_wf : forall var, unnatize_expr 0 (ExprEta' e (fun t => (nat * var t)%type)) = ExprEta' e _)
+             (Hwf : forall var1 var2,
+                 let P := (@reflect_wfT base_type base_type_eq_semidec_transparent op op_beq var1 var2 nil _ _ (ExprEta' e _) (ExprEta' e _)) in
+                 trueify P = P)
+             (** ** post-wf-pipeline *)
+             (Hpost : e_pkg = PostWfPipeline _ e input_bounds)
+             (Hpost_correct : Some {| input_expr := e ; input_bounds := input_bounds ; output_bounds := b ; output_expr := e' |} = e_pkg)
+             (** ** renaming *)
+             (Hrenaming : e_final = e')
+             (** ** bounds relaxation *)
+             (Hbounds_relax : Bounds.is_tighter_thanb b given_output_bounds = true)
+             (Hbounds_sane : pick_type given_output_bounds = pick_type b)
+             (Hbounds_sane_refl
+              : e_final_newtype
+                = eq_rect _ (fun t => Expr base_type op (Arrow (pick_type input_bounds) t)) e' _ (eq_sym Hbounds_sane))
+             (** ** instantiation of original evar *)
+             (Hevar : final_e_evar = InterpEta (t:=Arrow _ _) Syntax.interp_op e_final_newtype v')
+             (** ** side condition *)
+             (Hv : Bounds.is_bounded_by input_bounds (cast_back_flat_const v'))
+    : Bounds.is_bounded_by given_output_bounds (fZ (cast_back_flat_const v'))
+      /\ cast_back_flat_const final_e_evar = fZ (cast_back_flat_const v').
+  Proof.
+    destruct rexpr_sig as [? Hrexpr].
+    assert (Hwf' : Wf e)
+      by (apply (proj1 (@Wf_ExprEta'_iff _ _ _ e));
+          eapply reflect_Wf;
+          [ .. | intros; split; [ eapply He_unnatize_for_wf | rewrite <- Hwf; apply trueify_true ] ];
+          auto using base_type_eq_semidec_is_dec, op_beq_bl).
+    clear Hwf He_unnatize_for_wf.
+    symmetry in Hpost_correct.
+    subst; cbv [proj1_sig] in *.
+    rewrite eq_InterpEta, <- Hrexpr.
+    eapply PostWfPipelineCorrect in Hpost_correct; [ | solve [ eauto ].. ].
+    rewrite !@InterpPreWfPipeline in Hpost_correct.
+    unshelve eapply relax_output_bounds; try eassumption; [].
+    match goal with
+    | [ |- context[Interp _ (@eq_rect ?A ?x ?P ?k ?y ?pf) ?v] ]
+      => rewrite (@ap_transport A P _ x y pf (fun t e => Interp interp_op e v) k)
+    end.
+    rewrite <- transport_pp, concat_Vp; simpl.
+    apply Hpost_correct.
+  Qed.
+End with_round_up_list.
 
 (** ** Assembling the Pipeline, in Ltac *)
 (** The tactic [refine_with_pipeline_correct] uses the
@@ -217,7 +221,7 @@ Qed.
 Ltac refine_with_pipeline_correct :=
   lazymatch goal with
   | [ |- _ /\ ?castback ?fW = ?fZ ?arg ]
-    => let lem := open_constr:(@PipelineCorrect _ _ _ _ _ _ _ _ _ _ _ _) in
+    => let lem := open_constr:(@PipelineCorrect _ _ _ _ _ _ _ _ _ _ _ _ _) in
        simple refine (lem _ _ _ _ _ _ _ _ _ _ _ _);
        subst fW fZ
   end;
