src/Compilers/Z/Bounds/RoundUpLemmas.v
@@ -1,0 +1,34 @@
+Require Import Coq.omega.Omega.
+Require Import Crypto.Compilers.Z.Bounds.Interpretation.
+Require Import Crypto.Util.ZRange.
+Require Import Crypto.Util.Tactics.BreakMatch.
+Require Import Crypto.Util.NatUtil.
+
+Notation round_up_monotone_T round_up
+  := (forall x y,
+         (x <= y)%nat
+         -> match round_up x, round_up y with
+            | Some x', Some y' => (x' <= y')%nat
+            | None, None => True
+            | Some _, None => True
+            | None, Some _ => False
+            end)
+       (only parsing).
+
+Lemma round_up_to_in_list_monotone (allowable_lgsz : list nat)
+  : round_up_monotone_T (Bounds.round_up_to_in_list allowable_lgsz).
+Proof.
+  intros x y H.
+  induction allowable_lgsz as [|s ss].
+  { constructor. }
+  { unfold Bounds.round_up_to_in_list in *.
+    repeat match goal with
+           | _ => solve [ trivial ]
+           | _ => progress simpl in *
+           | _ => progress break_innermost_match_step
+           | _ => progress break_innermost_match_hyps_step
+           | [ H : ?leb _ _ = true |- _ ] => apply NPeano.Nat.leb_le in H
+           | [ H : ?leb _ _ = false |- _ ] => apply NPeano.Nat.leb_gt in H
+           | _ => omega *
+           end. }
+Qed.
